Remove tutorial code, add my code

examples/NSL/DY.NSL.Protocol.fst
@@ -9,159 +9,120 @@ open DY.Extend
 
 open DY.NSL.Data
 
-/// Here, we define the model of the 
-/// Needham-Schroeder-Lowe Fixed Public Key Protocol (NSL)
-///
-/// A -> B: enc{A, N_A}_B       Msg 1
-/// B -> A: enc{B, N_A, N_B}_A  Msg 2
-/// A -> B: enc{N_B}_B          Msg 3
-///
-/// The model consists of 4 functions,
-/// one for each protocol step:
-/// 1. Alice sends the first message to Bob (`send_msg1`)
-/// 2. Bob sends the second message to Alice (`send_msg2`)
-/// 3. Alice sends the third message to Bob (`send_msg3`)
-/// 4. Bob receives the third message from Alice (`receive_msg3`)
+val send_msg1:
+  (alice: principal) -> state_id -> (bob: principal) -> traceful(option(state_id & timestamp))
 
-(*** Sending the first message (Alice, n_a) ***)
-
-/// Alice sends the first message to Bob:
-/// * Alice generates a new nonce [n_a]
-/// * encrypts the message (Alice, n_a) for Bob
-/// * sends the encrypted message
-/// * stores n_a and Bob in a state (in a new session)
-/// The step returns the ID of the new state
-/// and the timestamp of the message on the trace
-/// The step fails, if
-/// encryption was not successful, i.e.,
-/// Alice does not have a public key of Bob.
-
-val send_msg1: principal -> principal -> state_id -> traceful (option (state_id & timestamp))
-let send_msg1 alice bob alice_public_keys_sid =
+let send_msg1 alice alice_public_keys_sid bob =
+  // Generate nonce
   let* n_a = gen_rand in
-  
-  let msg1 = Msg1 {alice; n_a} in 
+
+  let init_event = Initiating{alice; bob; n_a} in
+  trigger_event alice init_event;*  
+
+  // Assemble, encrypt and finally send initial message
+  let msg1 = Msg1 {alice; n_a} in
   let*? msg1_encrypted = pke_enc_for alice bob alice_public_keys_sid key_tag msg1 in
-  let* msg_ts = send_msg msg1_encrypted in
+  let* msg1_ts = send_msg msg1_encrypted in
 
-  let state = SentMsg1 {bob; n_a} in
-  let* sid = start_new_session alice state in
+  // Store local state, logging that sending worked successfully
+  let msg1_state = SentMsg1 {bob; n_a} in
+  // traceful as it starts a new session (that is logged on the trace)
+  let* sid = start_new_session alice msg1_state in
 
-  return (Some (sid, msg_ts))
+  return (Some (sid, msg1_ts))
 
-(*** Replying to a first message ***)
+val receive_msg1_and_send_msg2:
+  (bob: principal) -> state_id -> state_id -> (msg1_ts: timestamp) -> traceful (option (state_id & timestamp))
 
-/// Bob receives the first messages and replies:
-/// * read the message from the trace
-/// * decrypt the message to (Alice, n_a)
-/// * generate a new nonce [n_b]
-/// * encrypt the reply (Bob, n_a, n_b) for Alice
-/// * send the encrypted reply
-/// * store n_a, n_b and Alice in a state in a new session
-/// The step returns the ID of the new state
-/// and the timestamp of the reply on the trace.
-/// The step fails, if one of
-/// * decryption fails
-/// * the message is not of the right type, i.e., not a first message
-/// * encryption fails (for example, if Bob doesn't have a public key for Alice)
+let receive_msg1_and_send_msg2 bob bob_private_keys_sid bob_public_keys_sid msg1_ts=
+  let*? msg1_encrypted = recv_msg msg1_ts in
+  let*? msg1 = pke_dec_with_key_lookup #message_t bob bob_private_keys_sid key_tag msg1_encrypted in
+  guard_tr (Msg1? msg1);*?
 
-val receive_msg1_and_send_msg2: principal -> state_id -> state_id -> timestamp -> traceful (option (state_id & timestamp))
-let receive_msg1_and_send_msg2 bob bob_private_keys_sid bob_public_keys_sid msg_ts =
-  let*? msg = recv_msg msg_ts in
-
-  let*? msg1_ = pke_dec_with_key_lookup #message_t bob bob_private_keys_sid key_tag msg in
-  guard_tr (Msg1? msg1_);*?
-  let Msg1 msg1 = msg1_ in
+  let Msg1 msg1 = msg1 in
   let alice = msg1.alice in
   let n_a = msg1.n_a in
 
   let* n_b = gen_rand in
 
+  trigger_event bob (Responding1{alice; bob; n_a; n_b});*
+
   let msg2 = Msg2 {bob; n_a; n_b} in
   let*? msg2_encrypted = pke_enc_for bob alice bob_public_keys_sid key_tag msg2 in
   let* msg2_ts = send_msg msg2_encrypted in
 
-  let state = SentMsg2 {alice; n_a; n_b} in
-  let* sess_id = start_new_session bob state in
-  
-  return (Some (sess_id, msg2_ts))
+  let msg2_state = SentMsg2 {alice; n_a; n_b} in
+  let* sid_ = start_new_session bob msg2_state in
 
-(*** Sending the final message ***)
+  return (Some (sid_, msg2_ts))
 
+val receive_msg2_and_send_msg3:
+  (alice: principal) -> state_id -> state_id -> (msg2_ts: timestamp) -> traceful (option (state_id & timestamp))
 
-/// Alice receives the second messages and replies:
-/// * read the message from the trace
-/// * decrypt the message to (Bob, n_a, n_b)
-/// * encrypt the reply (n_b) for Bob
-/// * send the encrypted reply
-/// * store n_a, n_b and Bob in a state in the session related to Bob and n_a
-/// The step returns the ID of the new state
-/// and the timestamp of the reply on the trace.
-/// The step fails, if one of
-/// * decryption fails
-/// * the message is not of the right type, i.e., not a first message
-/// * encryption fails (for example, if Bob doesn't have a public key for Alice)
-/// * there is no prior session related to Bob and n_a
+let receive_msg2_and_send_msg3 alice alice_private_keys_sid alice_public_keys_sid msg2_ts=
+  let*? msg2_encrypted = recv_msg msg2_ts in
+  let*? msg2 = pke_dec_with_key_lookup #message_t alice alice_private_keys_sid key_tag msg2_encrypted in
+  guard_tr (Msg2? msg2);*?
 
-val receive_msg2_and_send_msg3: principal -> state_id -> state_id -> timestamp -> traceful (option (state_id & timestamp))
-let receive_msg2_and_send_msg3 alice alice_private_keys_sid alice_public_keys_sid msg_ts =
-  let*? msg = recv_msg msg_ts in
-
-  let*? msg2_ = pke_dec_with_key_lookup #message_t alice alice_private_keys_sid key_tag msg in
-  guard_tr (Msg2? msg2_);*?
-  let Msg2 msg2 = msg2_ in
+  let Msg2 msg2 = msg2 in
   let bob = msg2.bob in
   let n_a = msg2.n_a in
-  let n_b = msg2.n_b in
+  let n_b = msg2.n_b in 
 
-  let*? (sid, st) = lookup_state #state_t alice
-    (fun st -> 
-          SentMsg1? st
-      && (SentMsg1?.sentmsg1 st).n_a = n_a
-      && (SentMsg1?.sentmsg1 st).bob = bob
+  // Check whether Alice has inited a session w/ principal bob and nonce n_a
+  let*? (sid, current_state_alice) = lookup_state #state_t alice
+    (fun current_state_alice -> 
+          SentMsg1? current_state_alice
+      && (SentMsg1?.sentmsg1 current_state_alice).n_a = n_a
+      && (SentMsg1?.sentmsg1 current_state_alice).bob = bob
     ) in
-  guard_tr(SentMsg1? st);*?
-  
+  guard_tr(SentMsg1? current_state_alice);*?
 
   let msg3 = Msg3 {n_b} in
   let*? msg3_encrypted = pke_enc_for alice bob alice_public_keys_sid key_tag msg3 in
   let* msg3_ts = send_msg msg3_encrypted in
 
-  let state = SentMsg3 {bob; n_a; n_b} in
-  set_state alice sid state;*
-  
+  // IMPORTANT: the state shall *always* contain all knowledge up until that point as set_state overwrites and does not append
+  let msg3_state = SentMsg3 {bob; n_a; n_b} in
+  set_state alice sid msg3_state;*
+
   return (Some (sid, msg3_ts))
 
-(*** Receiving the final message ***)
+val receive_msg3:
+  (bob: principal) -> state_id -> (msg3_ts: timestamp) -> traceful (option state_id)
 
-/// Bob receives the reply from Alice:
-/// * read the message from the trace
-/// * decrypt the message to (n_b)
-/// * check if Bob previously sent n_b in some session
-/// * store completion of this session in a new state
-/// Returns the ID of the session that is marked as completed.
-/// The step fails, if one of
-/// * decryption fails
-/// * the message is not of the right type, i.e., not a reply
-/// * there is no prior session related to n_a
-
-val receive_msg3: principal -> state_id -> timestamp -> traceful (option state_id)
-let receive_msg3 bob bob_private_keys_sid msg3_ts =
-  let*? msg = recv_msg msg3_ts in
-  let*? msg3 = pke_dec_with_key_lookup #message_t bob bob_private_keys_sid key_tag msg in
+let receive_msg3 bob bob_private_keys_sid msg3_ts=
+  let*? msg3_encrypted = recv_msg msg3_ts in
+  let*? msg3 = pke_dec_with_key_lookup #message_t bob bob_private_keys_sid key_tag msg3_encrypted in
   guard_tr (Msg3? msg3);*?
+
+  (*let alice = (RcvdMsg3?.receivedmsg3 current_state_bob).alice in
+  let n_b = (RcvdMsg3?.receivedmsg3 current_state_bob).n_b in*)
+
   let Msg3 msg3 = msg3 in
   let n_b = msg3.n_b in
+  //let alice = msg3.alice in
 
-  let*? (sid, st) = lookup_state #state_t bob
-    (fun st -> 
-          SentMsg2? st
-      && (SentMsg2?.sentmsg2 st).n_b = n_b
+  let*? (sid_, current_state_bob) = lookup_state #state_t bob
+    (fun current_state_bob ->
+          SentMsg2? current_state_bob
+      && (SentMsg2?.sentmsg2 current_state_bob).n_b = n_b
+      //&& (SentMsg2?.sentmsg2 current_state_bob).alice = alice
     ) in
-  guard_tr(SentMsg2? st);*?
-  let alice = (SentMsg2?.sentmsg2 st).alice in
-  let n_a = (SentMsg2?.sentmsg2 st).n_a in
+  guard_tr (SentMsg2? current_state_bob);*?
 
-  set_state bob sid (ReceivedMsg3 {alice; n_a; n_b});*
+  let*? (sid, msg2) = lookup_state #state_t bob
+    (fun msg2 -> 
+          SentMsg2? msg2
+      && (SentMsg2?.sentmsg2 msg2).n_b = n_b
+    ) in
+  guard_tr(SentMsg2? msg2);*?
+  let n_a = (SentMsg2?.sentmsg2 msg2).n_a in
+  let alice = (SentMsg2?.sentmsg2 msg2).alice in
 
-  return (Some sid)
+  set_state bob sid_ (RcvdMsg3 {alice; n_a; n_b});*
+
+  return (Some sid_)
+
+// Helper function needed for the proofs
+let nonce_label alice bob = join (principal_label alice) (principal_label bob)
