examples/TwoMessage/DY.TwoMessage.Protocol.fst
@@ -1,46 +1,44 @@
-module DY.Online.Protocol
+module DY.TwoMessage.Protocol
 
 open Comparse
 open DY.Core
 open DY.Lib
 
-// Manually copied from tutorial-code repo to `utils/` for now
+// Manually copied from tutorial-code repo to utils/ for now
 open DY.Simplified
 open DY.Extend
 
-open DY.Online.Data
+open DY.TwoMessage.Data
 
 // Sending the ping msg
 val send_ping:
-  (alice: principal) -> state_id -> (bob: principal) ->
-  traceful (option (state_id & timestamp))
+  (alice: principal) -> (bob: principal) ->
+  traceful (state_id & timestamp)
 
-let send_ping alice alice_public_keys_sid bob =
+let send_ping alice bob =
   // Generate nonce
   let* n_a = gen_rand in
 
-  // Assemble, encrypt and then send ping
+  // Assemble, serialize and then send ping
   let ping = Ping {alice = alice; n_a = n_a} in
-  let*? ping_encrypted = pke_enc_for alice bob alice_public_keys_sid key_tag ping in
-  let* msg_ts = send_msg ping_encrypted in
+  let ping_wire = serialize message_t ping in
+  let* msg_ts = send_msg ping_wire in
 
   // Store the local state and start new session (traceful, serializing happens internally)
   let ping_state = SentPing {bob = bob; n_a = n_a} in
   let* sid = start_new_session alice ping_state in
 
-  return (Some (sid, msg_ts))
+  return (sid, msg_ts)
 
 // Receiving the ping msg and responding w/ an ACK
 val receive_ping_and_send_ack:
-  (bob:principal) -> state_id -> state_id -> (ping_ts:timestamp) ->
+  (bob:principal) -> (ping_ts:timestamp) ->
   traceful (option (state_id & timestamp))
 
-let receive_ping_and_send_ack bob bob_private_keys_sid bob_public_keys_sid msg_ts=
+let receive_ping_and_send_ack bob msg_ts=
   // Receive, parse and verify that it is actually a ping msg 
   let*? msg = recv_msg msg_ts in
-  let*? png = pke_dec_with_key_lookup #message_t bob bob_private_keys_sid key_tag msg in
-  
-  // Ensures that png is of type Ping, fails otherwise (causing the whole function to fail)
+  let*? png = return (parse message_t msg) in
   guard_tr (Ping? png);*?
 
   // Msg is actually a ping, access it
@@ -50,8 +48,7 @@ let receive_ping_and_send_ack bob bob_private_keys_sid bob_public_keys_sid msg_t
 
   // Sending the ACK
   let ack = Ack {n_a} in
-  let*? ack_encrypted = pke_enc_for bob alice bob_public_keys_sid key_tag ack in
-  let* ack_ts = send_msg ack_encrypted in
+  let* ack_ts = send_msg (serialize message_t ack) in
 
   let ack_state = SentAck {alice; n_a} in
   let* sess_id = start_new_session bob ack_state in
@@ -60,12 +57,12 @@ let receive_ping_and_send_ack bob bob_private_keys_sid bob_public_keys_sid msg_t
 
 // Receiving an ACK
 val receive_ack:
-  (alice: principal) -> state_id -> (ack_ts: timestamp) ->
+  (alice: principal) -> (ack_ts: timestamp) ->
   traceful (option state_id)
 
-let receive_ack alice alice_private_keys_sid ack_ts =
-  let*? msg = recv_msg ack_ts in
-  let*? ack = pke_dec_with_key_lookup #message_t alice alice_private_keys_sid key_tag msg in
+let receive_ack alice ack_ts =
+  let*? ack = recv_msg ack_ts in
+  let*? ack = return (parse message_t ack) in
   guard_tr (Ack? ack);*?
 
   let Ack ack = ack in
