examples/NSL/DY.NSL.Invariants.Proofs.fst
@@ -1,0 +1,125 @@
+module DY.NSL.Invariants.Proofs
+
+open Comparse
+open DY.Core
+open DY.Lib
+
+open DY.Simplified
+open DY.Extend
+
+open DY.NSL.Data
+open DY.NSL.Protocol
+open DY.NSL.Invariants
+
+// Taken from OnlineS
+//#set-options "--fuel 0 --ifuel 1 --z3rlimit 25  --z3cliopt 'smt.qi.eager_threshold=100'"
+
+// Customized options
+#set-options "--fuel 30 --ifuel 5 --z3rlimit 100  --z3cliopt 'smt.qi.eager_threshold=100'"
+
+val send_msg1_invariant:
+  alice:principal -> bob:principal -> alice_public_keys_sid:state_id -> tr:trace ->
+  Lemma
+  ( requires trace_invariant tr
+  )
+  (ensures (
+    let (_, tr_out) = send_msg1 alice alice_public_keys_sid bob tr in
+    trace_invariant tr_out
+  ))
+
+let send_msg1_invariant alice bob alice_public_keys_sid tr = 
+  let (n_a, tr_rand) = gen_rand_labeled (nonce_label alice bob) tr in
+  let (_, tr_out) = send_msg1 alice alice_public_keys_sid bob tr_rand in
+  assert(trace_invariant tr_rand);
+  //assert(trace_invariant tr_out);
+  // TODO: may mismatch with gen_rand
+  
+  //assert(trace_invariant tr_rand);
+  // The following line does not change the trace
+  let msg1 = Msg1 {alice; n_a} in
+  match pke_enc_for alice bob alice_public_keys_sid key_tag msg1 tr_rand with
+  | (None, tr_enc) -> (
+    assert(trace_invariant tr_rand);
+    assert(trace_invariant tr_enc);
+    assert(has_pki_invariant);
+    serialize_wf_lemma message_t (is_knowable_by (nonce_label alice bob) tr_enc) msg1;
+    serialize_wf_lemma message_t (is_knowable_by (nonce_label alice bob) tr_rand) msg1;
+    assume(tr_enc == tr_rand);
+    // This is the final goal for this case. Given that the encryption fails, tr_enc == tr_rand should also hold. Maybe we can use this to our advantage somehow. We cannot prove it as is however...
+    // TODO: get rid of the assumes
+    assume(tr == tr_enc);
+    admit()
+  )
+    // encryption failed, trace not interacted with
+  | (Some msg1_encrypted, tr_enc) -> (
+    assert(trace_invariant tr_enc);
+    let (msg_ts, tr_msg) = send_msg msg1_encrypted tr_enc in
+    assert(has_pki_invariant);
+    serialize_wf_lemma message_t (is_knowable_by (nonce_label alice bob) tr_rand) msg1;
+    let (pk_bob_opt, _) = get_public_key alice alice_public_keys_sid (LongTermPkeKey key_tag) bob tr_rand in
+    assert(None? pk_bob_opt \/
+      pke_pred.pred tr_rand (long_term_key_type_to_usage (LongTermPkeKey key_tag) bob) (Some?.v pk_bob_opt) (serialize message_t msg1)
+    );
+    pke_enc_for_is_publishable tr_rand alice bob alice_public_keys_sid key_tag msg1;
+    assert(trace_invariant tr_msg);
+
+    let st = SentMsg1 {bob; n_a} in
+    let (sid, tr_sess) = start_new_session alice st tr_msg in
+
+    assert(state_predicate_nsl.pred tr_msg alice sid st);
+    assert(trace_invariant tr_sess);
+    admit()
+  )
+
+  val receive_msg1_and_send_msg2:
+    alice:principal -> bob:principal -> bob_public_keys_sid:state_id -> bob_private_keys_sid:state_id -> msg1_ts:timestamp -> tr:trace ->
+    Lemma
+    (requires trace_invariant tr)
+    (ensures (
+      let (_, tr_out) = receive_msg1_and_send_msg2 bob bob_private_keys_sid bob_public_keys_sid msg1_ts in
+      trace_invariant tr_out
+    ))
+
+
+  let receive_msg1_and_send_msg2 alice bob bob_public_keys_sid bob_private_keys_sid msg1_ts tr = (
+    // receive msg1
+    let*? msg1 = recv_msg msg1_ts in
+    // decrypt ...
+    let*? msg1_d = pke_dec_with_key_lookup #message_t bob bob_private_keys_sid key_tag msg1 in
+    // ... check welformedness of msg1 ...
+    guard_tr (Msg1? msg1);*?
+    // ... and deconstruct
+    let Msg1 msg1 = msg1 in
+    let alice = msg1.alice in
+    let n_a = msg1.n_a in
+    // prepare  msg2
+    let (n_b, tr_rand) = gen_rand_labeled (nonce_label alice bob) tr_dec in
+    let (_, tr_out) = send_msg1 alice alice_public_keys_sid bob tr_rand in
+    // create msg2
+    let msg2 = Msg2 {bob; n_a; n_b} in
+    // encrypt msg2
+    // send msg2
+    admit()
+    )
+
+  val receive_msg2_and_send_msg3:
+    alice:principal -> bob:principal -> alice_public_keys_sid:state_id -> alice_private_keys_sid:state_id -> msg2_ts:timestamp -> tr:trace ->
+    Lemma
+    (requires trace_invariant tr)
+    (ensures (
+      let (_, tr_out) = receive_msg2_and_send_msg3 alice bob alice_private_keys_sid alice_public_keys_sid msg2_ts in
+      trace_invariant tr_out
+    ))
+
+  let receive_msg2_and_send_msg3 alice bob alice_public_keys_sid alice_private_keys_sid msg2_ts tr = (admit())
+
+  val receive_msg3:
+    alice:principal -> bob:principal -> bob_public_keys_sid:state_id -> bob_private_keys_sid:state_id -> msg3_ts:timestamp -> tr:trace ->
+    Lemma
+    (requires trace_invariant tr)
+    (ensures (
+      let (_, tr_out) = receive_msg3 alice bob bob_public_keys_sid bob_private_keys_sid msg3_ts in
+      trace_invariant tr_out
+    ))
+
+  let receive_msg3 alice bob bob_public_keys_sid bob_private_keys_sid msg3_ts tr = (admit())
