examples/NSL/DY.NSL.Invariants.fst
@@ -1,0 +1,197 @@
+module DY.NSL.Invariants
+
+open Comparse
+open DY.Core
+open DY.Lib
+open DY.Extend
+
+open DY.NSL.Data
+open DY.NSL.Protocol
+
+// may or may not be needed
+open FStar.List.Tot.Base
+
+// Taken from OnlineS
+#set-options "--fuel 0 --ifuel 1 --z3rlimit 25"
+
+(* Crypto invariants *)
+
+%splice [ps_msg1_t_is_well_formed] (gen_is_well_formed_lemma (`msg1_t))
+%splice [ps_msg2_t_is_well_formed] (gen_is_well_formed_lemma (`msg2_t))
+%splice [ps_msg3_t_is_well_formed] (gen_is_well_formed_lemma (`msg3_t))
+%splice [ps_message_t_is_well_formed] (gen_is_well_formed_lemma (`message_t))
+
+// Taken from OnlineS, not sure if needed
+instance crypto_usages_nsl : crypto_usages = default_crypto_usages
+
+#push-options "--ifuel 3"
+let crypto_predicates_nsl : crypto_predicates = {
+  default_crypto_predicates with
+  
+  pke_pred = {
+    pred = (fun tr sk_usage pk msg ->
+    (exists prin.
+      sk_usage == long_term_key_type_to_usage (LongTermPkeKey key_tag) prin /\
+      (match parse message_t msg with
+      | Some (Msg1 {alice; n_a}) ->
+        let bob = prin in
+        get_label tr n_a == nonce_label alice bob /\
+        event_triggered tr alice (Initiating {alice; bob; n_a})
+      | Some (Msg2 {bob; n_a; n_b}) ->
+        let alice = prin in
+        get_label tr n_a == nonce_label alice bob /\
+        get_label tr n_b == nonce_label alice bob /\
+        event_triggered tr bob (Responding1{alice; bob; n_a; n_b})
+      | Some (Msg3 {n_b}) ->
+        True // Analogous to just accepting a previously sent and verified nonce in the Online protocol
+      | _ -> False // fallthrough case, reject all other messages that do not conform to any of the expected types.
+      ))
+    );
+  pred_later = (fun tr1 tr2 sk_usage pk msg ->
+    parse_wf_lemma message_t (bytes_well_formed tr1) msg
+  );
+  };
+}
+#pop-options
+
+instance crypto_invariants_nsl: crypto_invariants = {
+  usages = crypto_usages_nsl;
+  preds = crypto_predicates_nsl
+}
+
+(* State invariants *)
+
+%splice [ps_sent_msg1_t_is_well_formed](gen_is_well_formed_lemma (`sent_msg1_t))
+%splice [ps_sent_msg2_t_is_well_formed](gen_is_well_formed_lemma (`sent_msg2_t))
+%splice [ps_sent_msg3_t_is_well_formed](gen_is_well_formed_lemma (`sent_msg3_t))
+%splice [ps_rcvd_msg3_t_is_well_formed](gen_is_well_formed_lemma (`rcvd_msg3_t))
+%splice [ps_state_t_is_well_formed](gen_is_well_formed_lemma (`state_t))
+
+#push-options "--ifuel 2 --z3cliopt 'smt.qi.eager_threshold=50'"
+let state_predicate_nsl: local_state_predicate state_t = {
+  pred = (fun tr prin sess_id st ->
+    match st with
+    | SentMsg1 {bob; n_a} -> (
+      let alice = prin in
+      is_secret (nonce_label alice bob) tr n_a /\
+      //is_knowable_by (nonce_label alice bob) tr n_a /\
+      event_triggered tr alice (Initiating{alice; bob; n_a})
+    )
+    | SentMsg2 {alice; n_a; n_b} -> (
+      let bob = prin in
+      //is_knowable_by (principal_label bob) tr n_a /\
+      is_secret (nonce_label alice bob) tr n_b /\
+      //is_knowable_by (nonce_label alice bob) tr n_b /\
+      event_triggered tr bob (Responding1{alice; bob; n_a; n_b}) /\
+      // Too strong of an assumption as is. If the attacker sends some public n_a, neither hold
+      ((is_secret (nonce_label alice bob) tr n_a /\
+      //is_knowable_by (nonce_label alice bob) tr n_a /\
+      state_was_set_some_id tr alice (SentMsg1 {bob; n_a})) \/
+      is_publishable tr n_a)
+    )
+    | SentMsg3 {bob; n_a; n_b} -> (
+      let alice = prin in
+      is_secret (nonce_label alice bob) tr n_a /\
+      //is_knowable_by (nonce_label alice bob) tr n_a /\
+      event_triggered tr alice (Initiating{alice; bob; n_a}) /\
+      ((is_secret (nonce_label alice bob) tr n_b /\
+      //is_knowable_by (nonce_label alice bob) tr n_b /\
+      state_was_set_some_id tr bob (SentMsg2 {alice; n_a; n_b})) \/
+      (is_publishable tr n_a /\ is_publishable tr n_b))
+    )
+    | RcvdMsg3 {alice; n_a; n_b} -> (
+      let bob = prin in
+      is_secret (nonce_label alice bob) tr n_b /\
+      //is_knowable_by (nonce_label alice bob) tr n_b /\
+      event_triggered tr bob (Responding1{alice; bob; n_a; n_b}) /\
+      ((is_secret (nonce_label alice bob) tr n_a /\
+      //is_knowable_by (nonce_label alice bob) tr n_a /\
+      state_was_set_some_id tr alice (SentMsg3 {bob; n_a; n_b})) \/
+      (is_publishable tr n_a ))
+    )
+    | _ -> False
+    );
+  pred_later = (fun tr1 tr2 prin sess_id st -> ());
+  pred_knowable = (fun tr prin sess_id st -> ());
+  (*
+  match st with
+  | RcvdMsg3 {alice; n_a; n_b} -> 
+    let bob = prin in
+    assert(is_knowable_by (principal_label prin) tr n_a);
+    assert(is_knowable_by (principal_label prin) tr n_b)    
+  | _ -> ()
+  );*)
+}
+#pop-options
+
+(*.Event invariants, taken from NSLP *)
+let event_predicate_nsl: event_predicate event_t =
+  fun tr prin e ->
+    match e with
+    | Initiating {alice; bob; n_a} -> (
+      prin == alice /\
+      is_secret (nonce_label alice bob) tr n_a /\
+      rand_just_generated tr n_a
+    )
+    | Responding1 {alice; bob; n_a; n_b} -> (
+      prin == bob /\
+      is_secret (nonce_label alice bob) tr n_b /\
+      rand_just_generated tr n_b
+    )
+
+(* Trace invariants *)
+
+let all_sessions = [
+  pki_tag_and_invariant;
+  private_keys_tag_and_invariant;
+  (|local_state_state_t.tag,
+  local_state_predicate_to_local_bytes_state_predicate
+  state_predicate_nsl|);
+]
+
+/// List of all local event predicates, taken from NSLP
+
+let all_events = [
+  (event_event_t.tag, compile_event_pred event_predicate_nsl)
+]
+
+let trace_invariants_nsl: trace_invariants = {
+  state_pred = mk_state_pred all_sessions;
+  event_pred = mk_event_pred all_events;
+}
+
+instance protocol_invariants_nsl: protocol_invariants = {
+  crypto_invs = crypto_invariants_nsl;
+  trace_invs = trace_invariants_nsl;
+}
+
+let complies_with_nsl_protocol tr = trace_invariant
+#protocol_invariants_nsl tr
+
+val all_sessions_has_all_sessions: unit -> Lemma (norm [delta_only [`%all_sessions; `%for_allP]; iota; zeta] (for_allP (has_local_bytes_state_predicate) all_sessions))
+let all_sessions_has_all_sessions () =
+  assert_norm(List.Tot.no_repeats_p (List.Tot.map dfst (all_sessions)));
+  mk_state_pred_correct all_sessions;
+  norm_spec [delta_only [`%all_sessions; `%for_allP]; iota; zeta] (for_allP (has_local_bytes_state_predicate) all_sessions)
+
+val protocol_invariants_p_has_p_session_invariant: squash (has_local_state_predicate state_predicate_nsl)
+let protocol_invariants_p_has_p_session_invariant = all_sessions_has_all_sessions ()
+
+val protocol_invariants_p_has_pki_invariant: squash (has_pki_invariant #protocol_invariants_nsl)
+let protocol_invariants_p_has_pki_invariant = all_sessions_has_all_sessions ()
+
+val protocol_invariants_p_has_private_keys_invariant: squash (has_private_keys_invariant #protocol_invariants_nsl)
+let protocol_invariants_p_has_private_keys_invariant = all_sessions_has_all_sessions ()
+
+/// Lemmas that the global event predicate contains all the local ones, taken from NSLP
+
+val all_events_has_all_events: unit -> Lemma (norm [delta_only [`%all_events; `%for_allP]; iota; zeta] (for_allP (has_compiled_event_pred #protocol_invariants_nsl) all_events))
+let all_events_has_all_events () =
+  assert_norm(List.Tot.no_repeats_p (List.Tot.map fst (all_events)));
+  mk_event_pred_correct #protocol_invariants_nsl all_events;
+  norm_spec [delta_only [`%all_events; `%for_allP]; iota; zeta] (for_allP (has_compiled_event_pred #protocol_invariants_nsl) all_events);
+  let dumb_lemma (x:prop) (y:prop): Lemma (requires x /\ x == y) (ensures y) = () in
+  dumb_lemma (for_allP (has_compiled_event_pred #protocol_invariants_nsl) all_events) (norm [delta_only [`%all_events; `%for_allP]; iota; zeta] (for_allP (has_compiled_event_pred #protocol_invariants_nsl) all_events))
+
+val protocol_invariants_nsl_has_nsl_event_invariant: squash (has_event_pred event_predicate_nsl)
+let protocol_invariants_nsl_has_nsl_event_invariant = all_events_has_all_events ()
