examples/NSL/DY.NSL.Properties.fst
@@ -1,0 +1,119 @@
+module DY.NSL.Properties
+
+open Comparse
+open DY.Core
+open DY.Lib
+open DY.Simplified
+open DY.Extend
+
+open DY.NSL.Data
+open DY.NSL.Invariants
+
+// Contains secrecy and authentication properties
+
+// We want both n_a and n_b to stay secret, i.e., be unknown to the attacker
+val n_a_secrecy:
+  tr:trace -> alice:principal -> bob:principal -> n_a:bytes -> n_b:bytes ->
+  Lemma
+  (requires
+    complies_with_nsl_protocol tr /\ (
+      (state_was_set_some_id tr alice (SentMsg1 {bob; n_a})) \/
+      (exists n_b. state_was_set_some_id tr bob (SentMsg2 {alice; n_a; n_b})) \/
+      (exists n_b. state_was_set_some_id tr alice (SentMsg3 {bob; n_a; n_b})) \/
+      (exists n_b. state_was_set_some_id tr bob (RcvdMsg3 {alice; n_a; n_b}))
+    )
+  )
+  (ensures
+    attacker_knows tr n_a ==>
+    principal_is_corrupt tr alice \/ principal_is_corrupt tr bob
+  )
+
+let nonce_label alice bob = join (principal_label alice) (principal_label bob)
+
+val publishable_implies_corruption:
+  tr:trace -> alice:principal -> bob:principal -> n:bytes ->
+  Lemma
+    (requires
+      trace_invariant tr /\
+      is_secret (nonce_label alice bob) tr n
+    )
+    (ensures 
+      is_publishable tr n ==>
+      principal_is_corrupt tr alice \/
+      principal_is_corrupt tr bob
+    )
+
+let publishable_implies_corruption tr alice bob n_a = ()
+
+let n_b_secrecy tr alice bob n_a n_b =
+  introduce attacker_knows tr n_a ==> principal_is_corrupt tr alice \/ principal_is_corrupt tr bob
+  with _ .
+    attacker_only_knows_publishable_values tr n_a
+
+(*
+let n_a_secrecy tr alice bob n_a n_b =
+  introduce attacker_knows tr n_a ==> principal_is_corrupt tr alice \/ principal_is_corrupt tr bob
+  with _ .
+    attacker_only_knows_publishable_values tr n_a*)
+
+val n_b_secrecy:
+  tr:trace -> alice:principal -> bob:principal -> n_a:bytes -> n_b:bytes ->
+  Lemma
+  (requires
+    complies_with_nsl_protocol tr /\ (
+      (state_was_set_some_id tr bob (SentMsg2 {alice; n_a; n_b})) \/
+      (state_was_set_some_id tr alice (SentMsg3 {bob; n_a; n_b}))
+    )
+  )
+  (ensures
+    attacker_knows tr n_b ==>
+    principal_is_corrupt tr alice \/ principal_is_corrupt tr bob
+  )
+
+let n_b_secrecy tr alice bob n_a n_b =
+  introduce attacker_knows tr n_b ==> principal_is_corrupt tr alice \/ principal_is_corrupt tr bob
+  with _ .
+    attacker_only_knows_publishable_values tr n_b
+
+// If Bob at the end of a run believes to be talking with Alice, then this Alice must indeed be involved in the run.
+val initiator_authentication:
+  alice:principal -> bob:principal -> n_a:bytes -> n_b:bytes -> tr:trace ->
+  Lemma
+  (requires
+    complies_with_nsl_protocol tr /\
+    trace_invariant tr /\
+    state_was_set_some_id tr bob (RcvdMsg3 {alice; n_a; n_b})
+  )
+  (ensures
+    principal_is_corrupt tr alice \/
+    principal_is_corrupt tr bob \/ (
+    state_was_set_some_id tr alice (SentMsg1 {bob; n_a}) /\
+    state_was_set_some_id tr alice (SentMsg3 {bob; n_a; n_b})
+    // TODO: Not sure if the following line is strictly necessary since it is implied by setting the RcvdMsg3 state
+    //state_was_set_some_id tr bob (SentMsg2 {alice; n_a; n_b})
+    )
+  )
+
+let initiator_authentication alice bob n_a n_b tr = ()
+  //assert(state_was_set_some_id tr alice (SentMsg3 {bob; n_a; n_b}))
+
+// If Alice at the end of a run believes to be talking with Bob, then this Bob must indeed be involved in the run.
+val responder_authentication:
+  alice:principal -> bob:principal -> n_a:bytes -> n_b:bytes -> tr:trace ->
+  Lemma
+  (requires
+    complies_with_nsl_protocol tr /\
+    trace_invariant tr /\
+    state_was_set_some_id tr alice (SentMsg3 {bob; n_a; n_b})
+  )
+  (ensures
+    principal_is_corrupt tr alice \/
+    principal_is_corrupt tr bob \/ (
+    state_was_set_some_id tr bob (SentMsg2 {alice; n_a; n_b})
+    //state_was_set_some_id tr bob (RcvdMsg3 {alice; n_a; n_b})
+    // Same as above: almost certainly not needed; bot from a proof perspective and to satisfy the intuitive meaning behind the statement
+    //state_was_set_some_id tr alice (SentMsg1 {bob; n_a})
+    )
+  )
+
+let responder_authentication alice bob n_a n_b tr = ()
