examples/NSL/DY.NSL.Run.Printing.fst
@@ -5,6 +5,7 @@ open DY.Lib
 open Comparse
 
 open DY.Simplified
+open DY.Extend
 
 open DY.NSL.Data
 
@@ -26,8 +27,8 @@ let state_to_string b =
   match? parse state_t b with
   | SentMsg1 s -> Some (Printf.sprintf "SentMsg1 [n_a = (%s), to = (%s)]" (bytes_to_string s.n_a) s.bob)
   | SentMsg2 s -> Some (Printf.sprintf "SentMsg2 [n_a = (%s), n_b = (%s), to = (%s)]" (bytes_to_string s.n_a) (bytes_to_string s.n_b) s.alice)
-  | SentMsg3 s -> Some (Printf.sprintf "SentMsg3 [n_a = (%s), n_b = (%s), to = (%s)]" (bytes_to_string s.n_a) (bytes_to_string s.n_b) s.bob)
-  | ReceivedMsg3 s -> Some (Printf.sprintf "ReceivedMsg3 [n_a = (%s), n_b = (%s), from = (%s)]" (bytes_to_string s.n_a) (bytes_to_string s.n_b) s.alice)
+  | SentMsg3 s -> Some (Printf.sprintf "SentMsg3 [n_b = (%s), to = (%s)]" (bytes_to_string s.n_b) s.bob)
+  | RcvdMsg3 s -> Some (Printf.sprintf "RcvdMsg3 [n_a = (%s), n_b = (%s), from = (%s)]" (bytes_to_string s.n_a) (bytes_to_string s.n_b) s.alice)
 
 
 val get_trace_to_string_printers: trace_to_string_printers
