examples/Online/DY.Online.Run.Printing.fst
@@ -3,9 +3,6 @@ module DY.Online.Run.Printing
 open DY.Core
 open DY.Lib
 open Comparse
-
-open DY.Simplified
-
 open DY.Online.Data
 
 /// Helper functions for trace printing.
@@ -15,20 +12,23 @@ open DY.Online.Data
 val message_to_string: bytes -> option string
 let message_to_string b =
   match? parse message_t b with
-  | Ping p -> Some (Printf.sprintf "Ping [name = (%s), n_a = (%s)]" (p.alice) (bytes_to_string p.n_a))
+  | Ping p -> Some (Printf.sprintf "Ping [name = (%s), n_a = (%s)]" (bytes_to_string p.n_a) p.alice)
   | Ack a -> Some (Printf.sprintf "Ack [n_a = (%s)]" (bytes_to_string a.n_a))
+
 
 val state_to_string: bytes -> option string
 let state_to_string b =
   match? parse state_t b with
   | SentPing p -> Some (Printf.sprintf "SentPing [n_a = (%s), to = (%s)]" (bytes_to_string p.n_a) p.bob)
-  | SentAck a -> Some (Printf.sprintf "SentAck [n_a = (%s), to = (%s)]" (bytes_to_string a.n_a) a.alice)
+  | SentAck a -> Some (Printf.sprintf "SentAck [n_a = (%s), to = (%s)]"  (bytes_to_string a.n_a) a.alice)
   | ReceivedAck r -> Some (Printf.sprintf "ReceivedAck [n_a = (%s), from = (%s)]" (bytes_to_string r.n_a) r.bob)
+
+
 
 
 val get_trace_to_string_printers: trace_to_string_printers
 let get_trace_to_string_printers  = 
   trace_to_string_printers_builder 
     message_to_string
-    ((local_state_state_t.tag, state_to_string) :: default_state_to_string)
+    [(local_state_state_t.tag, state_to_string)]
     []
