examples/TwoMessage/DY.TwoMessage.Run.fst
@@ -1,0 +1,31 @@
+module DY.TwoMessage.Run
+
+open DY.Core
+open DY.Lib
+open DY.Simplified
+
+open DY.TwoMessage.Protocol
+
+open DY.TwoMessage.Run.Printing
+
+val run:
+  unit -> traceful (option unit)
+let run () =
+  let alice = "Alice" in
+  let bob = "Bob" in
+
+  let* (alice_sid, ping_ts) = send_ping alice bob in
+  let*? (bob_sid, ack_ts) =
+    receive_ping_and_send_ack bob ping_ts in
+  receive_ack alice ack_ts;*?
+
+
+  let* tr = get_trace in
+  let _ = IO.debug_print_string "************* Trace *************\n" in
+  let _ = IO.debug_print_string (
+   trace_to_string get_trace_to_string_printers tr
+ ) in
+
+  return (Some ())
+
+let _ = run () empty_trace
